Work as of 10-04

AVL Tree.v
@@ -2,92 +2,93 @@ Require Export SfLib.
 
 Inductive tree: Type :=
 	| leaf : tree
-	| node : nat -> nat -> tree -> tree -> tree.
-	        (* Value -> Weight -> Left -> Right *)
-
-Check node 5 2 (node 3 0 leaf leaf) leaf.
+	| node : nat -> tree -> tree -> tree.
+	        (* Value -> Left -> Right *)
 
 Definition left (t: tree) := 
 	match t with
 	| leaf => None
-	| node _ _ leftChild _ => Some leftChild
+	| node _ leftChild _ => Some leftChild
 	end.
 
 Definition right (t: tree) := 
 	match t with
 	| leaf => None
-	| node _ _ _ rightChild => Some rightChild
+	| node _ _ rightChild => Some rightChild
 	end.
 
 
 Fixpoint height (t: tree) :=
 	match t with
 	| leaf => 0
-	| node _ _ leftChild rightChild => 1 + max (height leftChild) (height rightChild)
+	| node _ leftChild rightChild => 1 + max (height leftChild) (height rightChild)
 	end.
 
-
-Fixpoint insert (val:nat) (t: tree) := 
+Fixpoint add (val:nat) (t: tree) := 
 	match t with
-	| leaf => node val 0 leaf leaf
-	| node treeval weight lChild rChild => match ble_nat val treeval with
-										   | true => node treeval (weight+1) (insert val lChild) rChild
-										   | false => node treeval (weight-1) lChild (insert val rChild)
-										   end
+	| leaf => node val leaf leaf
+	| node treeval lChild rChild => 
+		match ble_nat val treeval with
+		| true => node treeval (add val lChild) rChild
+		| false => node treeval lChild (add val rChild)
+		end
 	end.
 
-Example insertexample:
-	insert 2 (insert 5 leaf) = node 5 1 (node 2 0 leaf leaf) leaf.
+Example addexample:
+	add 2 (add 5 leaf) = node 5 (node 2 leaf leaf) leaf.
 Proof. reflexivity. Qed.
 
 (*TODO: Look at weights *)
 Fixpoint balance (t : tree) :=
 	match t with
 	| leaf => leaf
-	| node val weight lChild rChild => 
-		match weight+2 with
+	| node val lChild rChild => 
+		match (height lChild) + 2 - (height rChild) with
 		| 0 => 
 			match rChild with
 			| leaf => leaf (* shouldn't happen *)
-			| node rval rweight rlChild rrChild => 
-				match rweight+2 with
-				| 1 => node rval (height (node val weight lChild rlChild) - height rrChild) (node val weight lChild rlChild) rrChild (* rr *)
+			| node rval rlChild rrChild => 
+				match (height rlChild) + 2 - (height rrChild) with
+				| 1 => node rval (node val lChild rlChild) rrChild (* rr *)
 				| _ => 
 					match rlChild with
-						| leaf => leaf (* shouldn't happen*)
-						| node rlval rlweight rllChild rlrChild => 
-							node rlval 0 (node val weight lChild rllChild) (node rval 0 rlrChild rrChild) (* rl *)
+					| leaf => leaf (* shouldn't happen*)
+					| node rlval rllChild rlrChild => 
+						node rlval (node val lChild rllChild) (node rval rlrChild rrChild) (* rl *)
 					end
 				end
 			end
 		| 4 => 
 			match lChild with
 			| leaf => leaf (* shouldn't happen *)
-			| node lval lweight llChild lrChild => 
-				match lweight+2 with
+			| node lval llChild lrChild => 
+				match (height llChild) + 2 - (height lrChild) with
 				| 1 => 
 					match lrChild with
 					| leaf => leaf (* shouldn't happen *)
-					| node lrval lrweight lrlChild lrrChild => 
-						node lrval 0 (node lval 0 llChild lrlChild) (node val 0 lrrChild rChild) (* lr *)
+					| node lrval lrlChild lrrChild => 
+						node lrval (node lval llChild lrlChild) (node val lrrChild rChild) (* lr *)
 					end
-				| _ => node lval 0 llChild (node val 0 lrChild rChild) (* ll *)
+				| _ => node lval llChild (node val lrChild rChild) (* ll *)
 				end
 			end
-		| _ => node val weight (balance lChild) (balance rChild)
+		| _ => node val (balance lChild) (balance rChild)
 		end
 	end.
 
+Definition insert val t :=
+	balance (add val t).
+
 Example leftexample :
-	left (node 3 1 leaf (node 2 0 leaf leaf)) = Some leaf.
+	left (node 3 leaf (node 2 leaf leaf)) = Some leaf.
 Proof. reflexivity. Qed.
 
 Example rightexample :
-	right (node 3 1 (node 2 0 leaf leaf) leaf) = Some leaf.
+	right (node 3 (node 2 leaf leaf) leaf) = Some leaf.
 Proof. reflexivity. Qed.
 
-Example insertexample :
-	insert 5 leaf = node 5 0 leaf leaf.
+Example add_example :
+	add 5 leaf = node 5 leaf leaf.
 Proof. reflexivity. Qed.
 	
 Example heightexample :
@@ -95,46 +96,39 @@ Example heightexample :
 Proof. reflexivity. Qed.
 
 Example heightexample2 :
-	height (node 5 1 leaf (node 3 0 leaf leaf)) = 2.
+	height (node 5 leaf (node 3 leaf leaf)) = 2.
 Proof. reflexivity. Qed.
 
 Fixpoint search (searchFor : nat) (t : tree) :=
 	match t with
 	| leaf => None
-	| node val _ leftChild rightChild => match beq_nat val searchFor with
-										| true => Some t
-										| false => match ble_nat searchFor val with
-												   | true => search searchFor leftChild
-												   | false => search searchFor rightChild
-												   end
-										end
+	| node val leftChild rightChild => 
+		match beq_nat val searchFor with
+		| true => Some t
+		| false => 
+			match ble_nat searchFor val with
+			| true => search searchFor leftChild
+			| false => search searchFor rightChild
+			end
+		end
 	end.
 
 Example searchexample :
-	search 5 (node 2 1 leaf (node 5 0 leaf leaf)) = Some (node 5 0 leaf leaf).
+	search 5 (node 2 leaf (node 5 leaf leaf)) = Some (node 5 leaf leaf).
 Proof. reflexivity. Qed.
 
 Example searchexample2 : 
 	search 5 leaf = None.
 Proof. reflexivity. Qed.
 
-Fixpoint wellformed (t: tree) :=
-	match t with
-	| leaf => true
-	| node val weight leftChild rightChild => match beq_nat weight ((height leftChild) - (height rightChild)) with
-												| false => false
-												| true => andb (wellformed leftChild) (wellformed rightChild)
-												end
-	end.
-
 Fixpoint inorder (t: tree) :=
 	match t with
 	| leaf => []
-	| node val _ leftChild rightChild => (inorder leftChild)++val::(inorder rightChild)
+	| node val leftChild rightChild => (inorder leftChild)++val::(inorder rightChild)
 	end.
 
 Definition Tree :=
-	 node 2 0 (node 1 0 leaf leaf) (node 5 0 leaf leaf).
+	 node 2 (node 1 leaf leaf) (node 5 leaf leaf).
 
 Example inorder_test :
 	inorder Tree = 1::2::5::[].
@@ -152,3 +146,56 @@ Proof. simpl. repeat apply more; try reflexivity. apply single. Qed.
 Example propnonsorted :
 	sorted (1::1::0::[]).
 Proof. apply more. reflexivity. apply more. (*UNPOSSIBLE!!!*) Admitted.
+
+Example balanced_tree :
+	insert 5 (insert 2 (insert 10 (insert 1 leaf))) = node 2 (node 1 leaf leaf) (node 10 (node 5 leaf leaf) leaf).
+Proof. reflexivity. Qed.
+
+Lemma sorted_app: forall l1 l2,
+	sorted(l1++l2) -> sorted l1 /\ sorted l2.
+Proof. 
+	intros. split. 
+		destruct l1. 
+			apply empty.
+			simpl in H. admit.
+		admit.
+Qed.
+
+Theorem insert_preserves_bst: forall n t,
+	sorted (inorder t) -> sorted (inorder (add n t)).
+Proof.
+	intros. induction t. 
+		Case "leaf". apply single.
+		Case "node". simpl in H. apply sorted_app in H. admit.
+Qed.
+
+Fixpoint pow base exponent :=
+	match exponent with
+	| 0 => 1
+	| S n => base * (pow base (n))
+	end.
+
+Example powcheck :
+	pow 5 2 = 25.
+Proof. reflexivity. Qed.
+
+Fixpoint log n c :=
+	match andb (ble_nat (pow 2 c) n) (negb (beq_nat (pow 2 c) n)) with
+	| false => c
+	| true => log n (c+1)
+	end.
+	
+Example log :
+	5*3 = 15.
+Proof. compute. reflexivity. Qed.
+
+Theorem insert_preserves_balance: forall n t t',
+	t = insert n t' -> height t = log2 (length (inorder t')+1).
+Proof. 
+	intros. induction t'.
+		Case "leaf". rewrite H. simpl. compute. reflexivity.
+		Case "node". rewrite H. simpl. destruct t'1. destruct t'2. simpl. compute.
+		
+Example justasmalltowngirl :
+	2+2=4.
+Proof. reflexivity. Qed.
